theories/core/utp_rel.thy
@@ -562,7 +562,7 @@ theorem SS2_DASHED_TWICE_app [urename]:
   apply (simp)
   apply (smt DASHED_TWICE_dash_elim dash_elim dash_undash_DASHED dash_undash_DASHED_TWICE f_inv_into_f o_def)
   apply (auto simp add:var_contra)
-  apply (metis dash_DASHED_image dash_UNDASHED_image image_compose)
+  apply (metis dash_DASHED_image dash_UNDASHED_image image_comp)
 done
 
 lemma SS2_DASHED_THRICE_app [urename]:
@@ -575,12 +575,12 @@ done
 theorem SS2_ident_app [urename]:
 "\<lbrakk>\<not> x \<in> UNDASHED; \<not> x \<in> DASHED_TWICE\<rbrakk> \<Longrightarrow> SS2\<bullet>x = x"
   apply (simp add:rename_on_rep_eq closure)
-  apply (metis (lifting, full_types) complete_inj_none dash_DASHED_image dash_UNDASHED_image image_compose)
+  apply (metis (lifting, full_types) complete_inj_none dash_DASHED_image dash_UNDASHED_image image_comp)
 done
 
 theorem SS2_VAR_RENAME_ON [closure] :
 "SS2 \<in> VAR_RENAME_ON (UNDASHED \<union> DASHED_TWICE)"
-  by (insert VAR_RENAME_ON_rename_on[of "dash \<circ> dash" UNDASHED, simplified], simp add:image_compose closure)
+  by (metis (no_types, hide_lams) UNDASHED_DASHED_inter(3) VAR_RENAME_ON_rename_on comp_rename_func dash_DASHED_image dash_DASHED_rename_func dash_UNDASHED_image dash_UNDASHED_rename_func image_comp order_refl)
 
 theorem SS2_VAR_RENAME_INV [closure] :
 "SS2 \<in> VAR_RENAME_INV"
@@ -601,7 +601,10 @@ theorem SS2_UNDASHED_DASHED_image [urename]:
 "\<lbrakk>vs \<subseteq> UNDASHED \<union> DASHED\<rbrakk> \<Longrightarrow>
  SS2 `\<^sub>s vs = dash ` dash ` (in vs) \<union> (out vs)"
   apply (simp only: rename_on_image closure)
-  apply (auto simp add:in_vars_def out_vars_def image_compose)
+  apply (simp add:in_vars_def out_vars_def)
+  apply (auto)
+  apply (metis DASHED_dash_elim IntI UnE contra_subsetD dash_DASHED_TWICE_elim dashed_twice_contras(2) imageI image_comp)
+  apply (metis IntI imageI image_comp undash_dash)
 done
 
 theorem SS2_UNDASHED_image [urename] :
@@ -618,7 +621,7 @@ done
 
 theorem SS2_DASHED_TWICE_image [urename] :
 "\<langle>SS2\<rangle>\<^sub>s ` DASHED_TWICE = UNDASHED"
-  by (metis (hide_lams, no_types) SS2_UNDASHED_image SS2_VAR_RENAME_INV VAR_RENAME_INV_comp' id_apply image_compose image_id)
+  by (metis (no_types, hide_lams) dash_DASHED_image dash_UNDASHED_image dash_dash_UNDASHED_rename_func image_comp order_refl rename_on_image2)
 
 theorem SS2_DASHED_THRICE_image [urename] :
 "\<langle>SS2\<rangle>\<^sub>s ` DASHED_THRICE = DASHED_THRICE"
