theories/utp_common.thy
@@ -11,8 +11,7 @@ theory utp_common
 imports utp_imports
   utp_document
   "core/utp_constants"
-(* Move the following into the theory utp_imports. *)
-  "utils/Unit_ord"
+  List_lexord
 begin
 
 default_sort type
@@ -26,7 +25,7 @@ text {* We are going to use the colon for type membership in UTP models. *}
 no_notation
   Set.member  ("op :") and
   Set.member  ("(_/ : _)" [51, 51] 50)
-
+  
 text {* The following prevents Isabelle from splitting pairs in proofs. *}
 
 declare split_paired_All [simp del]
